Source/DafnyCompilers/REPL/Repl.dfy
@@ -3,27 +3,64 @@ include "../CompilerCommon.dfy"
 include "../Printer.dfy"
 include "../Library.dfy"
 include "../CSharpDafnyASTModel.dfy"
+include "../CSharpDafnyInterop.dfy"
+include "../../AutoExtern/CSharpModel.dfy"
 
 import C = CSharpDafnyASTModel
-import D = DafnyCompilerCommon
+import DafnyCompilerCommon.AST
 import opened Lib.Datatypes
 
-type Expr = D.AST.Expr.Expr
+method {:extern "ParseExpression"} ParseExpression(s: System.String)
+  returns (e: C.Expression?)
 
-method {:extern "Read"} Read() returns (e: C.Expression)
+method {:extern "Input"} Input()
+  returns (e: System.String?)
 
-function method Translate(cE: C.Expression) : (o: Option<Expr>)
-  ensures o.Some? ==> Interp.SupportsInterp(o.t)
-  reads *
+datatype REPLError =
+  | ReadError
+  | ParseError
+  | InterpError(ie: Interp.InterpError)
+
+type REPLResult<+A> = Result<A, REPLError>
+
+method Read() returns (r: REPLResult<AST.Expr>)
+  ensures r.Success? ==> Interp.SupportsInterp(r.value)
 {
-  var e := D.Translator.TranslateExpression(cE);
-  if Interp.SupportsInterp(e) then Some(e) else None
+  var cStr := Input();
+  :- Need (cStr != null, ReadError);
+  :- Need (CSharpDafnyInterop.TypeConv.AsString(cStr) != "", ReadError);
+  var cExpr := ParseExpression(cStr);
+  :- Need (cExpr != null, ParseError);
+  var expr := DafnyCompilerCommon.Translator.TranslateExpression(cExpr);
+  :- Need(Interp.SupportsInterp(expr), InterpError(Interp.Unsupported(expr)));
+  return Success(expr);
 }
 
-function method Eval(e: Expr) : Values.T
+function method Eval(e: AST.Expr) : REPLResult<Values.T>
   requires Interp.SupportsInterp(e)
 {
-  Interp.InterpExpr(e).1
+  var OK(val, ctx) :- Interp.InterpExpr(e).MapFailure(e => InterpError(e)); // Map error
+  Success(val)
+}
+
+method ReadEval() returns (r: REPLResult<Values.T>) {
+  var expr :- Read();
+  var val :- Eval(expr);
+  return Success(val);
+}
+
+method ReportError(err: REPLError) {
+  match err
+    case ReadError => // Ignore silently
+    case ParseError => print "Parse error";
+    case InterpError(ie: Interp.InterpError) =>
+      print "Execution error: ";
+      match ie
+        case TypeError(e: Expr, value: V.T, expected: Type) => print "Type mismatch";
+        case InvalidExpression(e: Expr) => print "Invalid expression";
+        case Unsupported(e: Expr) => print "Unsupported expression";
+        case Overflow(x: int, low: int, high: int) => print "Overflow";
+        case DivisionByZero => print "Division by zero";
 }
 
 method Main()
@@ -32,11 +69,14 @@ method Main()
   while true
     decreases *
   {
-    var cExpr := Read();
-    match Translate(cExpr)
-      case None => print "Unsupported expression";
-      case Some(e) =>
-        var val := Eval(e);
+    print "∂~ ";
+    var r := ReadEval();
+    match r {
+      case Failure(err) =>
+        ReportError(err);
+      case Success(val) =>
         print Interp.Printer.ToString(val);
+    }
+    print "\n";
   }
 }
